# Solution to Review Question

by Qiang Gao, updated at June 8, 2018

---

## Chapter 2 Large-Sample Theory

### Section 1 Review of Limit Theorems for Sequences of Random Variables

...

#### Review Question 2.1.2 (Alternative definition of convergence for vector sequences)

(a) Verify that the definition in the text of “$$ \mathbf{z}_n \to_{m.s.} \mathbf{z} $$” is equivalent to

$$
\lim_{n \to \infty} \operatorname{E}
[ ( \mathbf{z}_n - \mathbf{z} )'( \mathbf{z}_n - \mathbf{z} ) ]
= 0.
$$

**Hint**: $$ \operatorname{E} [ ( \mathbf{z}_n - \mathbf{z} )'( \mathbf{z}_n - \mathbf{z} ) ] =
\operatorname{E} [ ( z_{n1} - z_1 )^2 ] + \cdots + 
\operatorname{E} [ ( z_{nK} - z_K )^2 ] $$, where $$K$$ is the dimension of $$\mathbf{z}$$.

(b) Similarly, verify that the definition in the text of “$$ \mathbf{z}_n \to_p \boldsymbol{\alpha} $$” is equivalent to

$$
\lim_{n \to \infty} \operatorname{Prob}
\left(
( \mathbf{z}_n - \boldsymbol{\alpha} )'
( \mathbf{z}_n - \boldsymbol{\alpha} ) >
\varepsilon
\right) = 0,
$$

for any $$ \varepsilon > 0 $$.

##### Solution

(a) If $$ \mathbf{z}_n \to_{m.s.} \mathbf{z} $$, by definition in the text,

$$
\lim_{n \to \infty} \operatorname{E}
[ ( z_{nk} - z_k )^2 ] = 0,
\text{ for $k = 1, \ldots, K$},
$$

then we can show

$$
\begin{align}
& \color{white}{=} \lim_{n \to \infty} \operatorname{E}
[ ( \mathbf{z}_n - \mathbf{z} )'( \mathbf{z}_n - \mathbf{z} ) ] \\
& = \lim_{n \to \infty}
\left(
\operatorname{E} [ ( z_{n1} - z_1 )^2 ] + \cdots + 
\operatorname{E} [ ( z_{nK} - z_K )^2 ]
\right) \\
& = \lim_{n \to \infty} \operatorname{E} [ ( z_{n1} - z_1 )^2 ] + \cdots + 
\lim_{n \to \infty} \operatorname{E} [ ( z_{nK} - z_K )^2 ] \\
& = 0.
\end{align}
$$

If $$ \lim_{n \to \infty} \operatorname{E}
[ ( \mathbf{z}_n - \mathbf{z} )'( \mathbf{z}_n - \mathbf{z} ) ] = 0 $$, then

$$
\lim_{n \to \infty} \operatorname{E} [ ( z_{n1} - z_1 )^2 ] + \cdots + 
\lim_{n \to \infty} \operatorname{E} [ ( z_{nK} - z_K )^2 ] = 0.
\tag{1}
$$

Because each terms in (1) are non-negative, (1) implies

$$
\lim_{n \to \infty} \operatorname{E}
[ ( z_{nk} - z_k )^2 ] = 0,
\text{ for $k = 1, \ldots, K$},
$$

which means $$ z_{nk} \to_{m.s.} z_k $$ for $$ k = 1, \ldots, K $$, and this implies $$ \mathbf{z}_n \to_{m.s.} \mathbf{z} $$ by definition in the text.

(b) Similarly, if $$ \mathbf{z}_n \to_p \boldsymbol{\alpha} $$, by definition in the text, for any $$ \varepsilon > 0 $$,

$$
\operatorname{Prob}
\left(
| z_{nk} - \alpha_k | > \varepsilon
\right) \to 0,
\text{ for $k = 1, \ldots, K$},
$$

then we can show

$$
\begin{gather}
\operatorname{Prob}
\left(
( z_{nk} - \alpha_k )^2 > \varepsilon^2
\right) \to 0,
\text{ for $k = 1, \ldots, K$}, 
&& \text{(equivalent event)} \\

\operatorname{Prob}
\left(
( z_{nk} - \alpha_k )^2 > \varepsilon
\right) \to 0,
\text{ for $k = 1, \ldots, K$},
&& \text{(any $\varepsilon > 0$)} \\

\operatorname{Prob}
\left(
( z_{n1} - \alpha_1 )^2 > \varepsilon
\right) + \cdots +
\operatorname{Prob}
\left(
( z_{nK} - \alpha_K )^2 > \varepsilon
\right) \to 0, 
&& \text{(limit sum)} \\

\left(
\not\Rightarrow
\operatorname{Prob}
\left(
(z_{n1} - \alpha_1)^2 + \cdots + (z_{nK} - \alpha_K)^2 > K \varepsilon
\right) \to 0
\right)
&& \text{(bigger event)} \\

\operatorname{Prob}
\left(
\bigcup_{k=1}^K
\left(
( z_{nk} - \alpha_k )^2 > \varepsilon
\right)
\right) \to 0, 
&& \text{(smaller event)} \\

\operatorname{Prob}
\left(
\bigcap_{k=1}^K
\left(
( z_{nk} - \alpha_k )^2 \leq \varepsilon
\right)
\right) \to 1, 
&& \text{(complement event)} \\

\operatorname{Prob}
\left(
( z_{n1} - \alpha_1 )^2 + \cdots +
( z_{nK} - \alpha_K )^2 \leq K \varepsilon
\right) \to 1, 
&& \text{(bigger event)} \\

\operatorname{Prob}
\left(
( z_{n1} - \alpha_1 )^2 + \cdots +
( z_{nK} - \alpha_K )^2 \leq \varepsilon
\right) \to 1,
&& \text{(any $\varepsilon > 0$)} \\

\operatorname{Prob}
\left(
( \mathbf{z}_n - \boldsymbol{\alpha} )'
( \mathbf{z}_n - \boldsymbol{\alpha} )
\leq \varepsilon
\right) \to 1, 
&& \text{(matrix notation)} \\

\operatorname{Prob}
\left(
( \mathbf{z}_n - \boldsymbol{\alpha} )'
( \mathbf{z}_n - \boldsymbol{\alpha} )
> \varepsilon
\right) \to 0.
&& \text{(complement event)}
\end{gather}
$$

If $$ \operatorname{Prob} \left( ( \mathbf{z}_n - \boldsymbol{\alpha} )' ( \mathbf{z}_n - \boldsymbol{\alpha} ) > \varepsilon \right) \to 0 $$, then we can show

$$
\begin{gather}
\operatorname{Prob}
\left(
( z_{n1} - \alpha_1 )^2 + \cdots +
( z_{nK} - \alpha_K )^2 > \varepsilon
\right) \to 0, 
&& \text{(scalar notation)} \\

\operatorname{Prob}
\left(
\bigcup_{k=1}^K
\left(
( z_{nk} - \alpha_k )^2 > \varepsilon
\right)
\right) \to 0, 
&& \text{(smaller event)} \\

\operatorname{Prob}
\left(
( z_{nk} - \alpha_k )^2 > \varepsilon
\right) \to 0
\text{ for $k = 1, \ldots, K$ },
&& \text{(smaller events)}
\end{gather}
$$

which means $$ z_{nk} \to_p \alpha_k $$ for $$ k = 1, \ldots, K $$, and this implies $$ \mathbf{z}_n \to_p \boldsymbol{\alpha} $$.

---

Copyright ©2018 by Qiang Gao